src/Examples/Interval/Example_Interval_DG_IP_Flagship.thy
@@ -220,7 +220,8 @@ proof -
              twice_transfer.tf_sound_enter_entry_for twice_transfer.tf_sound_combine_env_for
              ivl_tf_st_for_commute[folded fun_of_exec_dg_st_for_def]
              ivl_enter_st_for_commute[folded fun_of_exec_dg_st_for_def]
-             TD_side_warrowing_apinis_Interp.part_post_solution_of_solve_c)+
+             TD_side_warrowing_apinis_Interp.part_post_solution_of_solve_c
+        | assumption)+
 qed
 
 subsection \<open>Source-level soundness\<close>
