src/Examples/Sign/CallString/Example_Sign_DG_CallString_K1.thy
@@ -129,7 +129,8 @@ interpretation sign_nest_domain: routed_dg_domain_exec
   sign_nest_gs sign_nest_empty_pred "sign_tf_st_for sign_nest_gs"
   "sign_enter_st_for sign_nest_gs" "sign_tf_for sign_nest_gs"
   by unfold_locales
-     (rule sign_tf_st_for_commute, rule sign_enter_st_for_commute, rule sign_nest_exact)
+     (rule sign_tf_st_for_commute, assumption,
+      rule sign_enter_st_for_commute, rule sign_nest_exact)
 
 lemma sign_nest_gamma_eq: "sign_nest_gamma = sign_nest_domain.gamma_exec"
   by (intro ext) (simp add: sign_nest_gamma_def sign_nest_domain.gamma_exec_def gamma_dg_local_state_def)
